deps/poulet4/lib/LightTyping/CTK.v
@@ -1,0 +1,113 @@
+Require Import Poulet4.Ops Poulet4.Maps
+        Poulet4.Typed Poulet4.Value
+        Poulet4.Syntax Poulet4.Semantics
+        Poulet4.Monads.Monad Poulet4.Monads.Option
+        Poulet4.SyntaxUtil Poulet4.LightTyping.Utility.
+
+Notation path := (list String.string).
+
+(** * Compile-time Known Evaluation. *)
+
+Reserved Notation "'⟨' p ',' Σ ',' e '⟩' '⇝' v" (at level 80, no associativity).
+
+Inductive CTK_eval
+          {tags_t : Type}
+          (p : path)
+          (Σ : genv_const)
+  : @Expression tags_t -> @ValueBase bool -> Prop :=
+| CTK_bool i b τ d :
+    ⟨ p, Σ, MkExpression i (ExpBool b) τ d ⟩ ⇝ ValBaseBool b
+| CTK_num i n τ d :
+    ⟨ p, Σ, MkExpression i (ExpInt n) τ d ⟩ ⇝ eval_p4int_val n
+| CTK_const i x l τ v :
+    loc_to_val_const Σ p l = Some v ->
+    ⟨ p, Σ, MkExpression i (ExpName x l) τ Directionless ⟩ ⇝ v
+| CTK_uop i op e τ d v v' :
+    eval_unary_op op v = Some v' ->
+    ⟨ p, Σ, e ⟩ ⇝ v ->
+    ⟨ p, Σ, MkExpression i (ExpUnaryOp op e) τ d ⟩ ⇝ v'
+| CTK_bop i op e₁ e₂ τ d v v₁ v₂ :
+    eval_binary_op op v₁ v₂ = Some v ->
+    ⟨ p, Σ, e₁ ⟩ ⇝ v₁ ->
+    ⟨ p, Σ, e₂ ⟩ ⇝ v₂ ->
+    ⟨ p, Σ, MkExpression i (ExpBinaryOp op (e₁,e₂)) τ d ⟩ ⇝ v
+where "'⟨' p ',' Σ ',' e '⟩' '⇝' v" := (CTK_eval p Σ e v) : type_scope.
+
+Section CTKEval.
+  Context {tags_t: Type}.
+  Notation expr := (@Expression tags_t).
+  Notation Val := (@ValueBase bool).
+
+  Variables (p: path) (Σ: genv_const).
+
+  Fixpoint ctk_eval (e: expr) : option Val :=
+    match e with
+    | MkExpression _ (ExpBool b) _ _ => mret (ValBaseBool b)
+    | MkExpression _ (ExpInt  n) _ _ => mret (eval_p4int_val n)
+    | MkExpression
+        _ (ExpName _ l) _ Directionless => loc_to_val_const Σ p l
+    | MkExpression _ (ExpUnaryOp o e) _ _
+      => ctk_eval e >>= eval_unary_op o
+    | MkExpression _ (ExpBinaryOp o (e₁,e₂)) _ _
+      => let* v₁ := ctk_eval e₁ in
+        let* v₂ := ctk_eval e₂ in
+        eval_binary_op o v₁ v₂
+    | _ => None
+    end.
+
+  Local Hint Unfold option_bind : core.
+  
+  Lemma ctk_eval_complete : forall e v,
+      ⟨ p, Σ, e ⟩ ⇝ v -> ctk_eval e = Some v.
+  Proof.
+    intros e v H; induction H;
+      cbn in *; autounfold with core in *;
+        repeat match goal with
+               | H: ?trm = _ |- context [?trm]
+                 => rewrite H; clear H
+               end;
+        try reflexivity; auto.
+  Qed.
+
+  Local Hint Constructors CTK_eval : core.
+  
+  Lemma ctk_eval_sound : forall e v,
+      ctk_eval e = Some v -> ⟨ p, Σ, e ⟩ ⇝ v.
+  Proof.
+    intro e; induction e using expr_ind; intros v Hev;
+      cbn in *; autounfold with core in *;
+        try discriminate;
+        repeat match_some_inv; try some_inv; eauto.
+    - destruct dir; cbn in *; inv Hev; auto.
+    - destruct args as [e₁ e₂]; cbn in *;
+        repeat match_some_inv; eauto.
+  Qed.
+
+  Local Hint Constructors exec_expr : core.
+  Local Hint Unfold eval_val_to_sval : core.
+  Local Hint Unfold loc_to_sval_const : core.
+  Local Hint Unfold option_map : core.
+  Local Hint Resolve val_to_sval_ex : core.
+  Local Hint Resolve sval_to_val_eval_val_to_sval : core.
+  
+  Lemma CTK_exec_expr :
+    forall (T: Target) (gf: genv_func) (gt: genv_typ)
+      (gs: genv_senum) (gi: genv_inst) (ee: extern_env)
+      (rob : option bool -> bool -> Prop) (st : state)
+      (e : expr) (v : ValueBase),
+      (forall b, rob (Some b) b) ->
+      ⟨p,Σ,e⟩ ⇝ v ->
+      @exec_expr
+        _ T
+        {| ge_func:=gf; ge_typ:=gt; ge_senum:=gs;
+           ge_inst:=gi; ge_const:=Σ; ge_ext:=ee |}
+        rob p st e (ValueBaseMap Some v).
+  Proof.
+    intros T gf gt gs gi ee rob st e v Hrob H;
+      induction H; cbn in *; eauto.
+    - constructor; destruct n as [i' z [[w []] |]]; cbn; try reflexivity.
+    - apply exec_expr_name_const; cbn; try reflexivity.
+      autounfold with core; cbn.
+      rewrite H; reflexivity.
+  Qed.
+End CTKEval.
